examples/ring/CellHeader.v
@@ -3,11 +3,13 @@ Require Import Events Any IPM ImpPrelude IModL Skeleton.
 
 Module CellName.
 
-  Definition mk (idx: nat) (method: string) :=
-    "Cell" +:+ HexString.of_nat idx +:+ "." +:+ method.
+  Definition mn (idx: nat) := "Cell" +:+ HexString.of_nat idx.
+    
+  Definition fn (idx: nat) (method: string) :=
+    mn idx +:+ "." +:+ method.
   
-  Definition get idx := mk idx "get".
-  Definition set idx := mk idx "set".
+  Definition get idx := fn idx "get".
+  Definition set idx := fn idx "set".
 
 End CellName.
 
